Refinery/Term/Extrinsic/Wf/Swap.lean
@@ -85,6 +85,24 @@ theorem Eqv.let_comm_swap0 {A} {Γ Γl Γr : Ctx? α}
     ((a.wk0 ⟨B, 0⟩).let₁ ((hΓ.comm.s1_23_12 hΓc).comm.cons (.left _)) c.swap0)
   := by rw [Eqv.let_comm hΓ hΓc a b c he, swap0]
 
+theorem Eqv.let_pure_comm_swap0  {A} {Γ Γl Γr : Ctx? α}
+  (hΓ : Γ.SSplit Γc Γr) (hΓc : Γc.SSplit Γl Γm)
+  (a : Eqv R Γr A) (b : Eqv R Γm B) (c : Eqv R ((Γl.cons ⟨A, ⊤⟩).cons ⟨B, ⊤⟩) C)
+  [ha : a.HasEff ⊥]
+  : a.let₁ hΓ ((b.wk0 ⟨A, 0⟩).let₁ (hΓc.cons (.left _)) c)
+  = b.let₁ (hΓ.comm.s1_23_12_3 hΓc)
+    ((a.wk0 ⟨B, 0⟩).let₁ ((hΓ.comm.s1_23_12 hΓc).comm.cons (.left _)) c.swap0)
+  := let_comm_swap0 hΓ hΓc a b c (eb := ⊤) HasCommRel.commutes_bot_left
+
+theorem Eqv.let_comm_pure_swap0 {A} {Γ Γl Γr : Ctx? α}
+  (hΓ : Γ.SSplit Γc Γr) (hΓc : Γc.SSplit Γl Γm)
+  (a : Eqv R Γr A) (b : Eqv R Γm B) (c : Eqv R ((Γl.cons ⟨A, ⊤⟩).cons ⟨B, ⊤⟩) C)
+  [hb : b.HasEff ⊥]
+  : a.let₁ hΓ ((b.wk0 ⟨A, 0⟩).let₁ (hΓc.cons (.left _)) c)
+  = b.let₁ (hΓ.comm.s1_23_12_3 hΓc)
+    ((a.wk0 ⟨B, 0⟩).let₁ ((hΓ.comm.s1_23_12 hΓc).comm.cons (.left _)) c.swap0)
+  := let_comm_swap0 hΓ hΓc a b c (ea := ⊤) HasCommRel.commutes_bot_right
+
 theorem Eqv.wk2_swap0 {Γ : Ctx? α} {A B : Ty α} {x : Var? α} {y : Var? α} [hy : y.del]
   (a : Eqv R ((Γ.cons x).cons ⟨A, ⊤⟩) B)
   : a.swap0.wk2 y = (a.wk2 y).swap0
@@ -107,3 +125,58 @@ theorem Eqv.let₂_reswap
   apply Eq.trans _ (let₁_bv0 _)
   induction a, b using quotInd₂
   exact of_tm rfl
+
+def Eqv.swap0₂ {Γ : Ctx? α} {A B C : Ty α} {x : Var? α}
+  (a : Eqv R (((Γ.cons x).cons ⟨A, ⊤⟩).cons ⟨B, ⊤⟩) C)
+  : Eqv R (((Γ.cons ⟨A, ⊤⟩).cons ⟨B, ⊤⟩).cons x) C
+  := .let₁ Γ.erase_right.right.left.left .bv2
+      (.let₁ Γ.erase_right.left.right.left.left .bv2
+        ((a.wk3 _).wk3 _)
+      )
+
+def Eqv.unswap0₂ {Γ : Ctx? α} {A B C D : Ty α}
+  (a : Eqv R (((Γ.cons ⟨A, ⊤⟩).cons ⟨B, ⊤⟩).cons ⟨C, ⊤⟩) D)
+  : Eqv R (((Γ.cons ⟨C, ⊤⟩).cons ⟨A, ⊤⟩).cons ⟨B, ⊤⟩) D
+  :=  .let₁ Γ.erase_right.right.left.left .bv2 (a.wk3 _)
+
+-- theorem Eqv.let₂_let_comm_helper {A B C D : Ty α} {Γ Γl Γr : Ctx? α}
+--   (hΓ : Γ.SSplit Γc Γr) (hΓc : Γc.SSplit Γl Γm) {ea eb : ε}
+--   (a : Eqv R Γr (A.tensor B)) (b : Eqv R Γm C)
+--   (c : Eqv R (((Γl.cons ⟨A, ⊤⟩).cons ⟨B, ⊤⟩).cons ⟨C, ⊤⟩) D)
+--   [ha : a.HasEff ea] [hb : b.HasEff eb] [hc : c.HasEff ea] (he : ea ⇌ eb)
+--   : a.let₂ hΓ (((b.wk0 ⟨A, 0⟩).wk0 ⟨B, 0⟩).let₁ hΓc.left.left c)
+--   = b.let₁ (hΓ.comm.s1_23_12_3 hΓc)
+--     ((a.wk0 ⟨C, 0⟩).let₂ (hΓ.comm.s1_23_12 hΓc).comm.left c.unswap0₂)
+--   := by
+--   rw [unswap0₂]
+--   apply Eq.symm
+--   cases ha with
+--   | mk ha =>
+--   rename_i a
+--   cases hb with
+--   | mk hb =>
+--   rename_i b
+--   cases hc with
+--   | mk hc =>
+--   rename_i c
+--   apply Eqv.sound
+--   have hs :=
+--     Wf.pre_beta (B := D) (hΓ.comm.s1_23_12_3 hΓc) b 1 (by simp)
+--       ((a.wk0 ⟨C, 0⟩).let₂ (hΓ.comm.s1_23_12 hΓc).comm.left
+--         (.let₁ (Ctx?.erase_right _).right.left.left .bv2 (c.wk3 _)))
+--         (hb := sorry) he.symm (by simp; apply bot_le)
+--   apply hs.coh
+--   rfl
+--   simp [Wf.subst, Wf.let₂, Wf.let₁, Wf.wk0, Wf.wk3, Wf.bv2]
+--   constructor
+--   sorry
+--   sorry
+
+-- theorem Eqv.let₂_pair_left_wk0_wk0 {A B C D} {Γ Γc Γl Γm Γr : Ctx? α}
+--   (hΓ : Γ.SSplit Γc Γr) (hΓc : Γc.SSplit Γl Γm)
+--   (a : Eqv R Γr (.tensor A B)) (b : Eqv R Γl C) (c : Eqv R ((Γm.cons ⟨A, ⊤⟩).cons ⟨B, ⊤⟩) D)
+--   [ha : a.HasEff ea] [hb : b.HasEff eb] (he : ea ⇌ eb)
+--   : a.let₂ hΓ (.pair ((hΓc.cons (.right _)).cons (.right _)) ((b.wk0 _).wk0 _) c)
+--   = .pair (hΓ.s12_3_1_23 hΓc) b (.let₂ (hΓ.s12_3_23 hΓc) a c)
+--   := by
+--   sorry
